Semantics for shift operations

Graph/Values.thy
@@ -235,6 +235,64 @@ fun intval_abs :: "Value \<Rightarrow> Value" where
   "intval_abs (IntVal64 v) = (if (v) <s 0 then (IntVal64 (- v)) else (IntVal64 v))" |
   "intval_abs _ = UndefVal"
 
+lemma [code]: "shiftl1 n = n * 2"
+  by (simp add: shiftl1_eq_mult_2)
+
+lemma [code]: "shiftr1 n = n div 2"
+  by (simp add: shiftr1_eq_div_2)
+
+lemma [code]: "sshiftr1 n = word_of_int (sint n div 2)"
+  using sshiftr1_eq by blast
+
+definition shiftl (infix "<<" 75) where 
+  "shiftl w n = (shiftl1 ^^ n) w"
+
+lemma shiftl_power[simp]: "(x::('a::len) word) * (2 ^ j) = x << j"
+  unfolding shiftl_def apply (induction j)
+  apply simp unfolding funpow_Suc_right
+  by (metis (no_types, lifting) comp_def funpow_swap1 mult.left_commute power_Suc shiftl1_eq_mult_2)
+
+lemma "(x::('a::len) word) * ((2 ^ j) + 1) = x << j + x"
+  by (simp add: distrib_left)
+
+lemma "(x::('a::len) word) * ((2 ^ j) - 1) = x << j - x"
+  by (simp add: right_diff_distrib)
+
+lemma "(x::('a::len) word) * ((2^j) + (2^k)) = x << j + x << k"
+  by (simp add: distrib_left)
+
+lemma "(x::('a::len) word) * ((2^j) - (2^k)) = x << j - x << k"
+  by (simp add: right_diff_distrib)
+
+
+definition signed_shiftr (infix ">>" 75) where 
+  "signed_shiftr w n = (sshiftr1 ^^ n) w"
+
+definition shiftr (infix ">>>" 75) where 
+  "shiftr w n = (shiftr1 ^^ n) w"
+
+lemma shiftr_power[simp]: "(x::('a::len) word) div (2 ^ j) = x >>> j"
+  unfolding shiftr_def apply (induction j)
+  apply simp unfolding funpow_Suc_right
+  by (metis (no_types, lifting) comp_apply div_exp_eq funpow_swap1 power_Suc2 power_add power_one_right shiftr1_eq_div_2)
+
+
+
+fun intval_left_shift :: "Value \<Rightarrow> Value \<Rightarrow> Value" where
+  "intval_left_shift (IntVal32 v1) (IntVal32 v2) = IntVal32 (v1 << unat (v2 mod 32))" |
+  "intval_left_shift (IntVal64 v1) (IntVal64 v2) = IntVal64 (v1 << unat (v2 mod 64))" |
+  "intval_left_shift _ _ = UndefVal"
+
+fun intval_right_shift :: "Value \<Rightarrow> Value \<Rightarrow> Value" where
+  "intval_right_shift (IntVal32 v1) (IntVal32 v2) = IntVal32 (v1 >> unat (v2 mod 32))" |
+  "intval_right_shift (IntVal64 v1) (IntVal64 v2) = IntVal64 (v1 >> unat (v2 mod 64))" |
+  "intval_right_shift _ _ = UndefVal"
+
+fun intval_uright_shift :: "Value \<Rightarrow> Value \<Rightarrow> Value" where
+  "intval_uright_shift (IntVal32 v1) (IntVal32 v2) = IntVal32 (v1 >>> unat (v2 mod 32))" |
+  "intval_uright_shift (IntVal64 v1) (IntVal64 v2) = IntVal64 (v1 >>> unat (v2 mod 64))" |
+  "intval_uright_shift _ _ = UndefVal"
+
 (*
 end
 *)
