TheoryTesting.thy
@@ -44,6 +44,40 @@ lemma
   using assms unfolding valid_number.simps
   apply (simp add: Abs_IntegerHole_inverse)
   by (metis (no_types, hide_lams) bit.conj_disj_distrib2 bit.disj_cancel_left or.left_neutral word_ao_absorbs(2) word_oa_dist)
-  
+
+
+definition shiftl (infix "<<" 75) where 
+  "shiftl w n = (shiftl1 ^^ n) w"
+
+lemma shiftl_power[simp]: "(x::('a::len) word) * (2 ^ j) = x << j"
+  unfolding shiftl_def apply (induction j)
+  apply simp unfolding funpow_Suc_right
+  by (metis (no_types, lifting) comp_def funpow_swap1 mult.left_commute power_Suc shiftl1_eq_mult_2)
+
+lemma "(x::('a::len) word) * ((2 ^ j) + 1) = x << j + x"
+  by (simp add: distrib_left)
+
+lemma "(x::('a::len) word) * ((2 ^ j) - 1) = x << j - x"
+  by (simp add: right_diff_distrib)
+
+lemma "(x::('a::len) word) * ((2^j) + (2^k)) = x << j + x << k"
+  by (simp add: distrib_left)
+
+lemma "(x::('a::len) word) * ((2^j) - (2^k)) = x << j - x << k"
+  by (simp add: right_diff_distrib)
+
+
+definition signed_shiftr (infix ">>" 75) where 
+  "signed_shiftr w n = (sshiftr1 ^^ n) w"
+
+definition shiftr (infix ">>>" 75) where 
+  "shiftr w n = (shiftr1 ^^ n) w"
+
+lemma shiftr_power[simp]: "(x::('a::len) word) div (2 ^ j) = x >>> j"
+  unfolding shiftr_def apply (induction j)
+  apply simp unfolding funpow_Suc_right
+  by (metis (no_types, lifting) comp_apply div_exp_eq funpow_swap1 power_Suc2 power_add power_one_right shiftr1_eq_div_2)
+
+
 
 end
